Move embedding utility functions

embedding/theories/Utils.v
@@ -1,6 +1,7 @@
 From MetaCoq.Template Require Import All.
 From Coq Require Import String.
 From Coq Require Import List.
+From ConCert.Utils Require StringExtra.
 
 Import ListNotations.
 Import MCMonadNotation.
@@ -18,3 +19,76 @@ Fixpoint mkNames (prefix : string) (ns : list string) (postfix : string) :=
                   tmMkDefinition (TCString.of_string n) str;;
                   mkNames prefix ns' postfix
   end.
+
+Fixpoint mdots (prefix : modpath) (l : list MCString.string) :=
+  match l with
+  | [] => prefix
+  | h :: tl => mdots (MPdot prefix h) tl
+  end.
+
+(** Parses a string containing a file path and a module path
+    separated in a way that helps to recover the kername structure.
+ E.g. "Path/To/File#ModuleName.NestedModuleName" *)
+Definition modpath_of_string (s : string) : modpath :=
+  let fpath_mod := StringExtra.str_split "#" s in
+  let fpath := hd "" fpath_mod in
+  let module := hd "" (tl fpath_mod) in
+  let fpath_items := map TCString.of_string (rev (StringExtra.str_split "/" fpath)) in
+  let mod_items := map TCString.of_string (StringExtra.str_split "." module) in
+  let fp := MPfile fpath_items in
+  if module =? "" then fp
+  else mdots fp mod_items.
+
+(** Parses a string containing a file path, a module path separated
+    and a name in a way that helps to recover the kername structure.
+    E.g. "Path/To/File#ModuleName.NestedModuleName@FunctionName" *)
+Definition kername_of_string (s : string) : kername :=
+  let qualified_name := StringExtra.str_split "@" s in
+  if Nat.eqb (List.length qualified_name) 1
+  then (* unqualified name was given*)
+    (MPfile [], TCString.of_string (hd "" qualified_name))
+  else let path := hd "" qualified_name in
+       let name := TCString.of_string (hd "" (tl qualified_name)) in
+       (modpath_of_string path, name).
+
+(** The printing functions below are similar to the ones from MetaCoq,
+    but we use different separators for different parts of the [kername] *)
+Notation s_to_bs := bytestring.String.of_string.
+Definition string_of_dirpath (dp : dirpath) : string :=
+  TCString.to_string (TCString.concat (s_to_bs "/") (rev dp)).
+
+Fixpoint string_of_modpath (mp : modpath) : string :=
+  match mp with
+  | MPfile dp => string_of_dirpath dp
+  | MPbound dp id _ =>
+    (* currently not supported by the parser *)
+    (string_of_dirpath dp ++ "$" ++ (TCString.to_string id))%string
+  | MPdot mp0 id =>
+    match mp0 with
+    | MPfile _ => (string_of_modpath mp0 ++ "#" ++ (TCString.to_string id))%string
+    | _ => (string_of_modpath mp0 ++ "." ++ (TCString.to_string id))%string
+    end
+  end.
+
+Definition string_of_kername (kn : kername) :=
+  (string_of_modpath kn.1 ++ "@" ++ TCString.to_string kn.2)%string.
+
+Definition aRelevant (n : name) :=
+  {| binder_name := n; binder_relevance := Relevant |}.
+
+(** Extracts a constant name, inductive name or returns None *)
+Definition to_kername (t : Ast.term) : option kername :=
+  match t with
+  | Ast.tConst c _ => Some c
+  | Ast.tInd c _ => Some c.(inductive_mind)
+  | _ => None
+  end.
+
+Definition to_string_name (t : Ast.term) : string :=
+  match to_kername t with
+  | Some kn => string_of_kername kn
+  | None => "Not a constant or inductive"
+  end.
+
+Example qualified_bool : to_string_name (<% bool %>) = "Coq/Init/Datatypes@bool".
+Proof. reflexivity. Qed.
