embedding/examples/FinMap.v
@@ -31,7 +31,7 @@ Definition global_to_tc := compose trans_minductive_entry trans_global_dec.
 (** We generate names for inductives and constants (prefixed with a module path) *)
 MetaCoq Run
         (mp_ <- tmCurrentModPath tt ;;
-          let mp := (PCUICTranslate.string_of_modpath mp_ ++ "@")%string in
+          let mp := (Utils.string_of_modpath mp_ ++ "@")%string in
           mkNames mp ["Maybe"; "Map"] "Acorn").
 
 (** And constructors (just names, no module path prefix) *)
