embedding/extraction/SimpleBlockchainExt.v
@@ -25,8 +25,8 @@ Module AcornBlockchain.
   Definition Money := money.
 
   MetaCoq Run
-        ( mp_ <- tmCurrentModPath tt ;;
-          let mp := (PCUICTranslate.string_of_modpath mp_ ++ "@")%string in
+         (mp_ <- tmCurrentModPath tt ;;
+          let mp := (Utils.string_of_modpath mp_ ++ "@")%string in
           mkNames mp
                   ["SimpleChain" ; "Build_chain";
                   "SimpleContractCallContext" ; "Build_ctx" ;
