examples/crowdfunding/CrowdfundingExt.v
@@ -5,6 +5,7 @@ From ConCert.Embedding Require Import Notations.
 From ConCert.Embedding Require Import PCUICTranslate.
 From ConCert.Embedding Require Import TranslationUtils.
 From ConCert.Embedding Require Import Prelude.
+From ConCert.Embedding Require Import Utils.
 From ConCert.Embedding.Extraction Require Import Liquidity.
 From ConCert.Embedding.Extraction Require Import PreludeExt.
 From ConCert.Embedding.Extraction Require Import SimpleBlockchainExt.
